Simplified the data structure example side conditions
Simplified the side conditions arising from MiniML generation.  For
BottomUpMergeSort and RedBlackSet, the side conditions were either true in
general, or true when the data structure invariant is.  For the others, they all
simplified sown to something like x <> [] or x <> Empty.

examples/miniML/hol2miniml/okasaki-examples/BinomialHeapScript.sml
@@ -485,4 +485,15 @@ cases_on `q` >>
 rw [] >>
 metis_tac [delete_lem, merge_binomial_heap, remove_min_binomial_heap]);
 
+
+(* Simplify the side conditions on the generated certificate theorems *)
+
+val remove_min_tree_side_def = fetch "-" "remove_min_tree_side_def"
+val remove_min_tree_side_ind = fetch "-" "remove_min_tree_side_ind"
+
+val remove_min_tree_side = Q.prove (
+`!get_key leq h. remove_min_tree_side get_key leq h = (h ≠ [])`,
+recInduct remove_min_tree_side_ind >>
+rw [remove_min_tree_side_def]);
+
 val _ = export_theory ();
