examples/miniML/hol2miniml/okasaki-examples/LazyPairingHeapScript.sml
@@ -237,4 +237,19 @@ fs [delete_min_def, is_heap_ordered_def, merge_bag] >-
 metis_tac [merge_heap_ordered] >>
 rw [heap_to_bag_def, find_min_def, BAG_DIFF_INSERT2]);
 
+(* Simplify the side conditions on the generated certificate theorems *)
+
+val delete_min_side_def = fetch "-" "delete_min_side_def"
+val find_min_side_def = fetch "-" "find_min_side_def"
+
+val delete_min_side = Q.prove (
+`!get_key leq h. delete_min_side get_key leq h = (h ≠ Empty)`,
+cases_on `h` >>
+rw [delete_min_side_def]);
+
+val find_min_side = Q.prove (
+`!h. find_min_side h = (h ≠ Empty)`,
+cases_on `h` >>
+rw [find_min_side_def]);
+
 val _ = export_theory ();
